Fill all blanks

Leansubst/Basic.lean
@@ -13,6 +13,59 @@ variable (s t u : Subst σ)
 variable (i j k : Nat) (x : σ)
 variable (e : Expr σ) (es : List (Expr σ))
 
+def upr : Nat → (Nat → Nat) → (Nat → Nat)
+  | 0,     s => s
+  | i + 1, s => fun | 0 => 0 | k + 1 => (upr i s) k + 1
+
+def up : Nat → Subst σ → Subst σ
+  | 0,     s => s
+  | i + 1, s => cons (.var 0) (compr (up i s) (. + 1))
+
+theorem id_applyr : applyr (.) e = e := by
+  -- Induction on `e`.
+  apply @Expr.recOn _
+      (fun e => applyr (.) e = e)
+      (List.foldr (fun e etc => applyr (.) e = e ∧ etc) True)
+    <;> intros <;> (try trivial)
+  case var i => rw [applyr]
+  case binder e ih =>
+    conv => lhs; rw [applyr]
+    conv => rhs; rw [← ih]
+    congr 2; apply funext; intros k; cases k <;> rfl
+  case node x es ih =>
+    induction es with
+    | nil => simp only [applyr, applyr.nested]
+    | cons h' t' ih' =>
+      rw [List.foldr] at ih
+      simp only [applyr, applyr.nested] at *
+      congr 2
+      . exact ih.left
+      . specialize ih' ih.right
+        simp only [applyr, applyr.nested] at ih'
+        injection ih'
+
+theorem applyr_applyr (s r) : applyr r (applyr s e) = applyr (r ∘ s) e := by
+  revert s r
+  -- Induction on `e`.
+  let motive := fun (e : Expr σ) => ∀ s r, @applyr σ r (applyr s e) = applyr (r ∘ s) e
+  apply @Expr.recOn _ (fun e => motive e) (List.foldr (fun e etc => motive e ∧ etc) True)
+    <;> intros <;> (try trivial) <;> intros s t
+  case var i => rw [applyr, applyr, applyr]; rfl
+  case binder e ih =>
+    rw [applyr, applyr, applyr, ih]
+    congr 2; apply funext; intros k; cases k <;> rfl
+  case node x es ih =>
+    induction es with
+    | nil => simp only [applyr, applyr.nested]
+    | cons h' t' ih' =>
+      rw [List.foldr] at ih
+      simp only [applyr, applyr.nested] at *
+      congr 2
+      . exact ih.left _ _
+      . specialize ih' ih.right
+        simp only [applyr, applyr.nested] at ih'
+        injection ih'
+
 /-- `applyr` agrees with `apply` for renamings. -/
 @[simp high]
 theorem applyr_def (r) : @applyr σ r = apply (.var ∘ r) := by
@@ -21,12 +74,10 @@ theorem applyr_def (r) : @applyr σ r = apply (.var ∘ r) := by
   let motive := fun (e : Expr σ) => ∀ r, applyr r e = apply (.var ∘ r) e
   apply @Expr.recOn _ (fun e => motive e) (List.foldr (fun e etc => motive e ∧ etc) True)
     <;> intros <;> (try trivial) <;> intros r
-  case var k => rw [applyr, apply]; rfl
+  case var i => rw [applyr, apply]; rfl
   case binder e ih =>
-    rw [applyr, apply]; congr 2; rw [ih]
-    suffices h : (.var ∘ fun | 0 => 0 | i + 1 => r i + 1) =
-                 (cons (.var 0) (compr (.var ∘ r) (fun x => x + 1))) by rw [← h]; rfl
-    apply funext; intros i
+    rw [applyr, apply, ih]
+    congr 2; apply funext; intros i
     cases i with
     | zero => rfl
     | succ i => simp only [Function.comp, cons, compr, applyr]
@@ -48,37 +99,103 @@ theorem compr_def (s r) : @compr σ s r = comp s (.var ∘ r) := by
   apply funext; intros i
   rw [compr, comp, applyr_def]
 
-def up : Nat → Subst σ → Subst σ
-  | 0,     s => s
-  | i + 1, s => cons (.var 0) (compr (up i s) (1 + .))
+/-- Accessing higher entries of `upr`. -/
+theorem upr_get_high (r) : upr i r (i + j) = r j + i := by
+  induction i with
+  | zero => rw [Nat.zero_add]; rfl
+  | succ i ih => rw [Nat.succ_add, Nat.add_succ, ← ih]; rfl
 
-theorem gg : apply (up 1 s) (applyr (1 + .) e) = applyr (1 + .) (apply s e) := by
+/-- Accessing lower entries of `upr`. -/
+theorem upr_get_low (r) (h : j < i) : (upr i r) j = j := by
+  induction i generalizing j with
+  | zero => contradiction
+  | succ i ih =>
+    cases Nat.eq_or_lt_of_le (Nat.le_of_lt_succ h) with
+    | inl h' =>
+      subst h'; rw [upr]
+      cases j with
+      | zero => rfl
+      | succ j => simp only; rw [ih _ (Nat.lt_succ_self _)]
+    | inr h' =>
+      rw [upr]
+      cases j with
+      | zero => rfl
+      | succ k =>
+        simp only
+        rw [ih _ (Nat.le_of_lt_succ h)]
+
+/-- Accessing higher entries of `up`. -/
+theorem up_get_high : (up i s) (i + j) = applyr (. + i) (s j) := by
+  induction i with
+  | zero =>
+    rw [up, Nat.zero_add, funext Nat.add_zero, id_applyr]
+  | succ i ih =>
+    rw [up, Nat.succ_add, cons]; simp only
+    rw [compr, ih, applyr_applyr]; rfl
+
+/-- Accessing lower entries of `up`. -/
+theorem up_get_low (h : j < i) : (up i s) j = .var j := by
+  induction i generalizing j with
+  | zero => contradiction
+  | succ i ih =>
+    cases Nat.eq_or_lt_of_le (Nat.le_of_lt_succ h) with
+    | inl h' =>
+      subst h'; rw [up]
+      cases j with
+      | zero => rfl
+      | succ j =>
+        rw [cons]; simp only
+        rw [compr, ih _ (Nat.lt_succ_self _), applyr]
+    | inr h' =>
+      rw [up]
+      cases j with
+      | zero => rfl
+      | succ k =>
+        rw [cons]; simp only
+        rw [compr, ih _ (Nat.le_of_lt_succ h), applyr]
+
+/-- `upr` agrees with `up` for renamings. -/
+@[simp high]
+theorem upr_def (r) : .var ∘ upr i r = @up σ i (.var ∘ r) := by
+  apply funext; intros j
+  cases Nat.lt_sum_ge j i with
+  | inl h => rw [Function.comp, upr_get_low _ _ _ h, up_get_low _ _ _ h]
+  | inr h =>  
+    have ⟨d, hd⟩ := Nat.le.dest h; subst hd; clear h
+    rw [Function.comp, upr_get_high, up_get_high, Function.comp, applyr]
+
+/-- A difficult lemma for proving `apply_apply`... -/
+theorem gg : apply (up (i + 1) s) (applyr (upr i (. + 1)) e) = applyr (upr i (. + 1)) (apply (up i s) e) := by
   -- Induction on `e`.
-  let motive := fun (e : Expr σ) => ∀ s, @apply σ (up 1 s) (applyr (1 + .) e) = applyr (1 + .) (apply s e)
+  let motive := fun (e : Expr σ) => ∀ s i,
+      @apply σ (up (i + 1) s) (applyr (upr i (. + 1)) e) = applyr (upr i (. + 1)) (apply (up i s) e)
   apply @Expr.recOn _ (fun e => motive e) (List.foldr (fun e etc => motive e ∧ etc) True)
-    <;> intros <;> (try trivial) <;> intros s
-  case var k =>
-    simp only [Function.comp, apply]
+    <;> intros <;> (try trivial) <;> intros s i
+  case var j =>
+    rw [applyr, apply, apply]
+    cases Nat.lt_sum_ge j i with
+    | inl h => rw [up_get_low _ _ _ h, applyr, upr_get_low _ _ _ h, up_get_low _ _ _ (Nat.lt_succ_of_lt h)]
+    | inr h =>
+      have ⟨d, hd⟩ := Nat.le.dest h; subst hd; clear h
+      rw [up_get_high, upr_get_high, Nat.add_comm (d + 1), Nat.add_comm d, ← Nat.add_assoc, up_get_high, applyr_applyr]
+      congr 1; apply funext; intros j
+      rw [Function.comp, Nat.add_comm j i, upr_get_high, Nat.add_comm i 1, Nat.add_assoc]
   case binder e ih =>
-    simp [applyr_def, apply] at *
-    
-    rw [ih]
-    suffices h : (.var ∘ fun | 0 => 0 | i + 1 => r i + 1) =
-                 (cons (.var 0) (compr (.var ∘ r) (fun x => x + 1))) by rw [← h]; rfl
-    apply funext; intros i
-    cases i with
-    | zero => rfl
-    | succ i => simp only [Function.comp, cons, compr, applyr]
+    conv => lhs; rw [applyr, apply, ← up]
+    have h : s = up 0 s := rfl
+    conv => rhs; rw [apply, applyr, h, ← up]
+    congr 1
+    exact ih _ _
   case node x es ih =>
     induction es with
-    | nil => simp only [apply, apply.nested]
+    | nil => simp only [apply, apply.nested, applyr, applyr.nested]
     | cons h' t' ih' =>
       rw [List.foldr] at ih
-      simp only [apply, apply.nested] at *
+      simp only [apply, apply.nested, applyr, applyr.nested] at *
       congr 2
       . exact ih.left _ _
       . specialize ih' ih.right
-        simp only [apply, apply.nested] at ih'
+        simp only [apply, apply.nested, applyr, applyr.nested] at ih'
         injection ih'
 
 /-!
@@ -87,29 +204,33 @@ theorem gg : apply (up 1 s) (applyr (1 + .) e) = applyr (1 + .) (apply s e) := b
 -/
 
 @[simp]
-theorem get_zero : (cons e s) 0 = e := rfl
+theorem cons_zero : (cons e s) 0 = e := rfl
 
 @[simp]
-theorem get_succ : (cons e s) (i + 1) = s i := rfl
+theorem cons_succ : (cons e s) (i + 1) = s i := rfl
 
+/-- Normalise expanded `applyr`, `compr` and `upr`. -/
 @[simp]
-theorem shift_wrap_left : .var ∘ (i + .) = shift σ i := rfl
+theorem shift_wrap_right : .var ∘ (. + i) = shift σ i := rfl
 
+/-- Normalise expanded `applyr`, `compr` and `upr`. -/
 @[simp]
-theorem shift_wrap_right : .var ∘ (. + i) = shift σ i := by
+theorem shift_wrap_left : .var ∘ (i + .) = shift σ i := by
   apply funext; intros k; rw [Function.comp, Nat.add_comm]; rfl
 
+/-- Normalise `shift n` to either `shift 1` or `id`. -/
 @[simp]
 theorem shift_zero : shift σ 0 = id σ := by
   apply funext; intros i
-  rw [id, shift, Nat.zero_add]
+  rw [id, shift]; rfl
 
+/-- Normalise `shift n` to either `shift 1` or `id`. -/
 @[simp]
 theorem shift_succ_succ : shift σ (i + 1 + 1) = comp (shift σ (i + 1)) (shift σ 1) := by
-  apply funext; intros k
+  apply funext; intros j
   simp only [shift, comp, apply]
   conv => lhs; rw [Nat.add_comm i 1]
-  rw [Nat.add_assoc 1, Nat.add_assoc 1]
+  rw [Nat.add_comm 1 i, ← Nat.add_assoc]
 
 @[simp]
 theorem apply_var : apply s (.var i) = s i := by
@@ -127,6 +248,33 @@ theorem apply_node : apply s (.node x es) = .node x (es.map (apply s)) := by
   | cons h t ih => rw [List.map, apply, apply.nested] at *; congr 2; injection ih
 
 @[simp]
+theorem id_apply : apply (id σ) e = e := by
+  -- Induction on `e`.
+  apply @Expr.recOn _
+      (fun e => apply (id σ) e = e)
+      (List.foldr (fun e etc => apply (id σ) e = e ∧ etc) True)
+    <;> intros <;> (try trivial)
+  case var i => rw [apply]; rfl
+  case binder e ih =>
+    conv => lhs; rw [apply]
+    conv => rhs; rw [← ih]
+    congr 2; apply funext; intros k
+    cases k with
+    | zero => rfl
+    | succ => simp only [cons, id, compr, applyr]
+  case node x es ih =>
+    induction es with
+    | nil => simp only [apply, apply.nested]
+    | cons h' t' ih' =>
+      rw [List.foldr] at ih
+      simp only [apply, apply.nested] at *
+      congr 2
+      . exact ih.left
+      . specialize ih' ih.right
+        simp only [apply, apply.nested] at ih'
+        injection ih'
+
+@[simp]
 theorem apply_apply : apply t (apply s e) = apply (comp s t) e := by
   rw [comp_def]
   revert t s
@@ -134,23 +282,13 @@ theorem apply_apply : apply t (apply s e) = apply (comp s t) e := by
   let motive := fun (e : Expr σ) => ∀ s t, @apply σ t (apply s e) = (apply (apply t ∘ s)) e
   apply @Expr.recOn _ (fun e => motive e) (List.foldr (fun e etc => motive e ∧ etc) True)
     <;> intros <;> (try trivial) <;> intros s t
-  case var k => simp only [Function.comp, apply]
+  case var i => rw [apply, apply]; rfl
   case binder e ih =>
-    simp only [Function.comp, apply]
-    rw [ih]
-    simp [Function.comp]
-    suffices h :
-        apply (cons (.var 0) (apply (shift _ 1) ∘ t)) ∘ cons (.var 0) (apply (shift _ 1) ∘ s) =
-        cons (.var 0) (apply (shift _ 1) ∘ apply t ∘ s) by rw [h]
-    apply funext; intros i
+    rw [apply, apply, apply, ih]
+    congr 2; apply funext; intros i
     cases i with
     | zero => rfl
-    | succ i =>
-      suffices h : ∀ e,
-          apply (cons (.var 0) (compr t (1 + .))) (applyr (1 + .) e) =
-          applyr (1 + .) (apply t e) by
-        rw [applyr_def, compr_def] at h; exact h (s i)
-      exact gg _
+    | succ i => have h := gg t 0; rw [up, upr] at h; exact h (s i)
   case node x es ih =>
     induction es with
     | nil => simp only [apply, apply.nested]
@@ -164,40 +302,31 @@ theorem apply_apply : apply t (apply s e) = apply (comp s t) e := by
         injection ih'
 
 @[simp]
-theorem id_apply : apply (id σ) e = e := by
-  sorry
-
-@[simp]
 theorem id_comp : comp (id σ) s = s := by
-  sorry
+  apply funext; intros i; rw [comp_def, Function.comp, id, apply]
 
 @[simp]
 theorem comp_id : comp s (id σ) = s := by
-  sorry
+  apply funext; intros i; rw [comp_def, Function.comp, id_apply]
 
 @[simp]
 theorem shift_comp_cons : comp (shift σ 1) (cons e s) = s := by
-  sorry
+  apply funext; intros i; rw [comp_def, Function.comp, shift, apply]; rfl
 
 @[simp]
 theorem cons_comp : comp (cons e s) t = cons (apply t e) (comp s t) := by
-  sorry
+  apply funext; intros i; rw [comp_def, Function.comp, comp_def]; cases i <;> rfl
 
 @[simp]
 theorem comp_assoc : comp (comp s t) u = comp s (comp t u) := by
-  sorry
+  apply funext; intros i; simp only [comp_def, Function.comp, apply_apply]
 
 @[simp]
 theorem apply_zero_cons_shift_comp : cons (apply s (.var 0)) (comp (shift σ 1) s) = s := by
-  sorry
+  apply funext; intros i; cases i <;> rfl
 
 @[simp]
 theorem zero_cons_shift : cons (.var 0) (shift σ 1) = id σ := by
-  sorry
-
-/-
-example : comp (shift σ 1) (id σ) = shift σ 1 := by
-  simp
--/
+  apply funext; intros i; cases i <;> rfl
 
 end Leansubst.Subst
